engine/lib/iterator_expr.ml
@@ -1,0 +1,63 @@
+open! Prelude
+
+module Make (F : Features.T) = struct
+  module U = Ast_utils.Make (F)
+  module AST = Ast.Make (F)
+  open AST
+
+  type kind =
+    | Range of { min : expr; max : expr }
+    | Enumerate of t
+    | Zip of t * t
+    | ChunksExact of { it : t; size : expr }
+    | Indexable of expr  (** a slice, an array *)
+
+  and t = { kind : kind; typ : ty }
+
+  module Expect = struct
+    include U.Expect
+
+    let ( <|> ) (type a) (type b) (f: a -> b option) (g: a -> b option) x = match f x with Some r -> Some r | None -> g x
+
+    let any_ref (typ : ty) : ty option =
+      match typ with TRef { typ; _ } -> Some typ | _ -> None
+
+    let array (typ : ty) : ty option =
+      match typ with TArray { typ; _ } -> Some typ | _ -> None
+
+    let slice (typ : ty) : ty option =
+      match typ with TSlice { ty; _ } -> Some ty | _ -> None
+
+    let into_iter : expr -> expr option =
+      fun e -> concrete_app1 Core__iter__traits__collect__IntoIterator__into_iter e
+
+    let concrete_app_n (f : Concrete_ident.name) (e : expr) : expr list option =
+      match e.e with
+      | App { f = { e = GlobalVar (`Concrete f'); _ }; args; _ }
+        when Concrete_ident.eq_name f f' ->
+          Some args
+      | _ -> None
+
+    let concrete_app2 (f : Concrete_ident.name) (e : expr) :
+        (expr * expr) option =
+      match concrete_app_n f e with
+      | Some [ x; y ] -> Some (x, y)
+      | _ -> None
+
+    let indexable (e : expr) : t option =
+      let* e = into_iter e in
+      let* typ =
+        any_ref e.typ |> Option.value ~default:e.typ |> (array <|> slice)
+      in
+      Some { kind = Indexable e; typ }
+
+    let range (e : expr) : t option =
+      let* e = into_iter e in
+      let* min, max = concrete_app2 Core__ops__range__Range e in
+      Some { kind = Range { min; max }; typ = min.typ }
+  end
+
+  (* let from (e: expr): t option = *)
+  (*                              match e with *)
+  (*                            | Core__iter__traits__collect__IntoIterator__into_iter *)
+end
