engine/lib/phases/phase_reconstruct_for_index_loops.mli
@@ -1,0 +1,18 @@
+open! Prelude
+
+module Make (F : Features.T) : sig
+  include module type of struct
+    module FA = F
+
+    module FB = struct
+      include F
+      include Features.On.For_index_loop
+    end
+
+    module A = Ast.Make (F)
+    module B = Ast.Make (FB)
+    module ImplemT = Phase_utils.MakePhaseImplemT (A) (B)
+  end
+
+  include ImplemT.T
+end
