tests/attributes/src/lib.rs
@@ -1,9 +1,22 @@
-pub trait Foo: Clone {
-    fn foo(&self) -> Self;
-}
-
-impl Foo for u64 {
-    fn foo(&self) -> Self {
-        self.clone()
+fn hello(x: &mut [u8]) {
+    let y = &[10, 20, 30, 40];
+    let mut aa = 3;
+    aa += 1;
+    for i in 0..x.len() {
+        let lhs = x[i];
+        let rhs = y[i];
+        x[i] = lhs + rhs;
     }
 }
+
+fn main() -> u8 {
+    let mut x: [u8; 4] = [1, 2, 3, 4];
+    hello(&mut x);
+    let x1 = x[1];
+    let x0 = x[0];
+    x[0] = x1 + x0;
+    x[0]
+}
+
+// TODO list:
+// plus_u8
