proof-libs/fstar/core/Core.Ops.Index.IndexMut.fst
@@ -1,14 +1,34 @@
 module Core.Ops.Index.IndexMut
 
+
+open LowStar.BufferOps
+module B = LowStar.Buffer
+module HS = FStar.HyperStack
+module HST = FStar.HyperStack.ST
+
+
 class t_IndexMut t_Self t_Idx = {
-  f_Input: Type;
+  out_type: Type0;
   in_range: t_Self -> t_Idx -> Type0;
-  f_index_mut: s:t_Self -> i:t_Idx{in_range s i} -> v:f_Input -> t_Self;
+  f_index_mut: s:t_Self -> i:t_Idx{in_range s i} -> HST.St out_type;
 }
 
 open Rust_primitives
-instance impl__index_mut t l n: t_IndexMut (t_Array t l) (int_t n)
-  = { f_Input = t;
+instance impl__index_mut_array t l n: t_IndexMut (t_Array t l) (int_t n)
+  = { out_type = B.pointer t;
       in_range = (fun (s: t_Array t l) (i: int_t n) -> v i >= 0 && v i < v l);
-      f_index_mut = (fun s i x -> Seq.upd s (v i) x);
+      f_index_mut = (fun s i -> 
+        admit ();
+        B.sub s (cast i) 1ul
+      );
     }
+
+instance impl__index_mut_slice t n: t_IndexMut (t_Slice t) (int_t n)
+  = { out_type = B.pointer t;
+      in_range = (fun (s: t_Slice t) (i: int_t n) -> v i >= 0 && v i < v (spec_length s));
+      f_index_mut = (fun (Some s) i -> 
+        admit ();
+        B.sub s.buffer (cast i) 1ul
+      );
+    }
+
