proof-libs/fstar/core/Core.Ops.Range.fsti
@@ -8,10 +8,16 @@ type t_RangeFull           = | RangeFull
 
 open Core.Iter.Traits.Iterator
 
+open LowStar.BufferOps
+module B = LowStar.Buffer
+module HS = FStar.HyperStack
+module HST = FStar.HyperStack.ST
+
+
 let rec fold_range' #t
   (min: Rust_primitives.int_t t) (max: Rust_primitives.int_t t {v min <= v max})
-  (init: 'a) (f: ('a -> i:Rust_primitives.int_t t{v i < v max /\ v i >= v min} -> 'a))
-  : Tot 'a (decreases (v max - v min))
+  (init: 'a) (f: ('a -> i:Rust_primitives.int_t t{v i < v max /\ v i >= v min} -> HST.St 'a))
+  : HST.St 'a (decreases (v max - v min))
   = if min = max
     then init
     else fold_range' (add min (Rust_primitives.mk_int 1)) max (f init min) f
@@ -39,54 +45,83 @@ open Core.Ops.Index
 instance impl_index_range_slice t n : t_Index (t_Slice t) (t_Range (int_t n)) 
   = { f_Output = t_Slice t
     ; in_range = (fun (s: t_Slice t) {f_start; f_end} -> 
-         let len = Rust_primitives.length s in
+         let len = Rust_primitives.spec_length s in
          v f_start >= 0 /\ v f_start <= v len /\ v f_end <= v len)
     ; f_index = (fun s {f_start; f_end} -> 
-          if f_start <. f_end then Seq.slice s (v f_start) (v f_end)
-                              else Seq.empty)}
+          if f_start <. f_end 
+          then
+            let len = f_end -. f_start in
+            let Some s = s in
+            admit ();
+            let buffer: B.buffer t = B.sub s.buffer (cast f_start) (Ghost.hide (cast len)) in
+            let len: B.buffer usize = B.alloca (cast len <: usize) 1ul in
+            Some {buffer; len}
+          else None
+          )
+       }
 
 instance impl_index_range_to_slice t n : t_Index (t_Slice t) (t_RangeTo (int_t n)) 
   = { f_Output = t_Slice t
     ; in_range = (fun (s: t_Slice t) ({f_end}: t_RangeTo (int_t n)) -> 
-         let len = Rust_primitives.length s in v f_end <= v len)
-    ; f_index = (fun s {f_end} -> if 0 < v f_end then Seq.slice s 0 (v f_end) else Seq.empty)}
+         let len = Rust_primitives.spec_length s in v f_end <= v len)
+    ; f_index = admit ()}
+    // ; f_index = (fun s {f_end} -> if 0 < v f_end then Seq.slice s 0 (v f_end) else Seq.empty)}
 
 instance impl_index_range_from_slice t n : t_Index (t_Slice t) (t_RangeFrom (int_t n)) 
-  = { f_Output = t_Slice t
-    ; in_range = (fun (s: t_Slice t) ({f_start}: t_RangeFrom (int_t n)) -> 
-         let len = Rust_primitives.length s in v f_start >= 0 /\ v f_start <= v len)
-    ; f_index = (fun s {f_start} -> 
-         let len = Rust_primitives.length s in
-         if v f_start = v len then Seq.empty else Seq.slice s (v f_start) (v len))}
+   = admit ()
+//   = { f_Output = t_Slice t
+//     ; in_range = (fun (s: t_Slice t) ({f_start}: t_RangeFrom (int_t n)) -> 
+// <<<<<<< Updated upstream
+//          let len = Rust_primitives.length s in v f_start >= 0 /\ v f_start <= v len)
+//     ; f_index = (fun s {f_start} -> 
+//          let len = Rust_primitives.length s in
+//          if v f_start = v len then Seq.empty else Seq.slice s (v f_start) (v len))}
          
 instance impl_index_range_full_slice t : t_Index (t_Slice t) t_RangeFull
-  = { f_Output = t_Slice t
-    ; in_range = (fun (s: t_Slice t) _ -> True)
-    ; f_index = (fun s _ -> s)}
+         = admit ()
+//   = { f_Output = t_Slice t
+//     ; in_range = (fun (s: t_Slice t) _ -> True)
+//     ; f_index = (fun s _ -> s)}
+// ||||||| Stash base
+//          let len = Rust_primitives.length s in v f_start >= 0 /\ v f_start <= v len)
+//     ; f_index = (fun s {f_start} -> 
+//          let len = Rust_primitives.length s in
+//          if v f_start = v len then Seq.empty else Seq.slice s (v f_start) (v len))}
+// =======
+//          let len = Rust_primitives.spec_length s in v f_start >= 0 /\ v f_start <= v len)
+//     // ; f_index = (fun s {f_start} -> 
+//     ; f_index = (fun s {f_start} -> admit ())}
+//     //      let len = Rust_primitives.spec_length s in
+//     //      if v f_start = v len then Seq.empty else Seq.slice s (v f_start) (v len))}
+// >>>>>>> Stashed changes
 
 instance impl_range_index_array t len n : t_Index (t_Array t len) (t_Range (int_t n)) = 
   let i = impl_index_range_slice t n in
-  { f_Output = i.f_Output
-  ; in_range = (fun (s: t_Array t len) r -> i.in_range s r)
-  ; f_index = (fun s r -> i.f_index s r) }
+  admit ()
+  // { f_Output = i.f_Output
+  // ; in_range = (fun (s: t_Array t len) r -> i.in_range s r)
+  // ; f_index = (fun s r -> i.f_index s r) }
   
 instance impl_range_to_index_array t len n : t_Index (t_Array t len) (t_RangeTo (int_t n)) = 
   let i = impl_index_range_to_slice t n in
-  { f_Output = i.f_Output
-  ; in_range = (fun (s: t_Array t len) r -> i.in_range s r)
-  ; f_index = (fun s r -> i.f_index s r) }
+  admit ()
+  // { f_Output = i.f_Output
+  // ; in_range = (fun (s: t_Array t len) r -> i.in_range s r)
+  // ; f_index = (fun s r -> i.f_index s r) }
 
 instance impl_range_from_index_array t len n : t_Index (t_Array t len) (t_RangeFrom (int_t n)) = 
-  let i = impl_index_range_from_slice t n in
-  { f_Output = i.f_Output
-  ; in_range = (fun (s: t_Array t len) r -> i.in_range s r)
-  ; f_index = (fun s r -> i.f_index s r) }
+  admit ()
+  // let i = impl_index_range_from_slice t n in
+  // { f_Output = i.f_Output
+  // ; in_range = (fun (s: t_Array t len) r -> i.in_range s r)
+  // ; f_index = (fun s r -> i.f_index s r) }
 
 instance impl_range_full_index_array t len : t_Index (t_Array t len) t_RangeFull = 
   let i = impl_index_range_full_slice t in
-  { f_Output = i.f_Output
-  ; in_range = (fun (s: t_Array t len) r -> i.in_range s r)
-  ; f_index = (fun s r -> i.f_index s r) }
+  admit ()
+  // { f_Output = i.f_Output
+  // ; in_range = (fun (s: t_Array t len) r -> i.in_range s r)
+  // ; f_index = (fun s r -> i.f_index s r) }
 
 open Rust_primitives.Hax
 
@@ -112,19 +147,81 @@ val update_at_array_range_full t l n
   (s: t_Array t l) (i: t_RangeFull)
   : (update_at_tc_array_range_full_super t l n).f_Output -> t_Array t l
 
-instance update_at_tc_array_range t l n: update_at_tc (t_Array t l) (t_Range (int_t n)) = {
-  super_index = update_at_tc_array_range_super t l n;
-  update_at = update_at_array_range t l n
-}
-instance update_at_tc_array_range_to t l n: update_at_tc (t_Array t l) (t_RangeTo (int_t n)) = {
-  super_index = update_at_tc_array_range_to_super t l n;
-  update_at = update_at_array_range_to t l n
-}
-instance update_at_tc_array_range_from t l n: update_at_tc (t_Array t l) (t_RangeFrom (int_t n)) = {
-  super_index = update_at_tc_array_range_from_super t l n;
-  update_at = update_at_array_range_from t l n
-}
-instance update_at_tc_array_range_full t l n: update_at_tc (t_Array t l) t_RangeFull = {
-  super_index = update_at_tc_array_range_full_super t l n;
-  update_at = update_at_array_range_full t l n
-}
+// <<<<<<< updated upstream
+// instance update_at_tc_array_range t l n: update_at_tc (t_Array t l) (t_Range (int_t n)) = {
+//   super_index = update_at_tc_array_range_super t l n;
+//   update_at = update_at_array_range t l n
+// }
+// instance update_at_tc_array_range_to t l n: update_at_tc (t_Array t l) (t_RangeTo (int_t n)) = {
+//   super_index = update_at_tc_array_range_to_super t l n;
+//   update_at = update_at_array_range_to t l n
+// }
+// instance update_at_tc_array_range_from t l n: update_at_tc (t_Array t l) (t_RangeFrom (int_t n)) = {
+//   super_index = update_at_tc_array_range_from_super t l n;
+//   update_at = update_at_array_range_from t l n
+// }
+// instance update_at_tc_array_range_full t l n: update_at_tc (t_Array t l) t_RangeFull = {
+//   super_index = update_at_tc_array_range_full_super t l n;
+//   update_at = update_at_array_range_full t l n
+// }
+// ||||||| Stash base
+// instance update_at_tc_array_range t l n: update_at_tc (t_Array t l) (t_Range (int_t n)) = {
+//   super_index = update_at_tc_array_range_super t l n;
+//   update_at = update_at_array_range t l n
+// }
+// instance update_at_tc_array_range_to t l n: update_at_tc (t_Array t l) (t_RangeTo (int_t n)) = {
+//   super_index = update_at_tc_array_range_to_super t l n;
+//   update_at = update_at_array_range_to t l n
+// }
+// instance update_at_tc_array_range_from t l n: update_at_tc (t_Array t l) (t_RangeFrom (int_t n)) = {
+//   super_index = update_at_tc_array_range_from_super t l n;
+//   update_at = update_at_array_range_from t l n
+// }
+// =======
+// // instance update_at_tc_array_range t l n: update_at_tc (t_Array t l) (t_Range (int_t n)) = {
+// //   super_index = update_at_tc_array_range_super t l n;
+// //   update_at = update_at_array_range t l n
+// // }
+// // instance update_at_tc_array_range_to t l n: update_at_tc (t_Array t l) (t_RangeTo (int_t n)) = {
+// //   super_index = update_at_tc_array_range_to_super t l n;
+// //   update_at = update_at_array_range_to t l n
+// // }
+// // instance update_at_tc_array_range_from t l n: update_at_tc (t_Array t l) (t_RangeFrom (int_t n)) = {
+// //   super_index = update_at_tc_array_range_from_super t l n;
+// //   update_at = update_at_array_range_from t l n
+// // }
+// >>>>>>> Stashed changes
+
+
+open Rust_primitives.Integers
+
+instance impl__index_mut_array t l n: t_IndexMut (t_Array t l) (t_Range (int_t n))
+  = { out_type = t_Slice t;
+      in_range = (fun (s: t_Array t l) (i: t_Range (int_t n)) -> True);
+      f_index_mut = (fun s {f_start; f_end} -> 
+           if f_end >=. f_start
+           then
+             ( admit ();
+               let len = f_end -! f_start in
+               let buffer = B.sub s f_start len in
+               Some {buffer; len})
+           else None
+      );
+    }
+
+instance impl__index_mut_slice t n: t_IndexMut (t_Slice t) (t_Range (int_t n))
+  = { out_type = t_Slice t;
+      in_range = (fun (s: t_Slice t) (i: t_Range (int_t n)) -> True);
+      f_index_mut = (fun s {f_start; f_end} -> 
+        match s with
+        | None -> None
+        | Some s ->
+           if f_end >=. f_start
+           then
+             ( admit ();
+               let len = f_end -! f_start in
+               let buffer = B.sub s.buffer f_start len in
+               Some {buffer; len})
+           else None
+      );
+    }
