proof-libs/fstar/rust_primitives/Rust_primitives.Arrays.fst
@@ -2,19 +2,55 @@ module Rust_primitives.Arrays
 
 open Rust_primitives.Integers
 
-type t_Slice t = s:Seq.seq t{Seq.length s <= max_usize}
-type t_Array t (l:usize) = s: Seq.seq t { Seq.length s == v l }
+open LowStar.BufferOps
+module B = LowStar.Buffer
+module HS = FStar.HyperStack
+module HST = FStar.HyperStack.ST
 
-let of_list (#t:Type) (l: list t {FStar.List.Tot.length l < maxint Lib.IntTypes.U16}): t_Slice t = Seq.seq_of_list l
-let to_list (#t:Type) (s: t_Slice t): list t = Seq.seq_to_list s
+noeq type t_nonempty_Slice t = {
+   buffer: B.buffer t;
+   len:    len: usize {len == B.len buffer}
+}
+// Use Low* null thing
+inline_for_extraction type t_Slice t = option (t_nonempty_Slice t)
+inline_for_extraction type t_Array t (l:usize) = b: B.buffer t {B.length b = v l}
 
-let to_of_list_lemma t l = Seq.lemma_list_seq_bij l
-let of_to_list_lemma t l = Seq.lemma_seq_list_bij l
+inline_for_extraction
+let of_list (#t:Type) (l: list t {
+    FStar.List.Tot.length l < maxint Lib.IntTypes.U16
+  /\ FStar.List.Tot.length l > 0
+  })
+  : HST.StackInline 
+    (t_Array t (mk_int (FStar.List.Tot.length l)))
+    (requires fun _ -> True)
+    (requires fun h0 b h1 -> B.alloc_post_mem_common b h0 h1 (Seq.seq_of_list l)
+                        /\ B.frameOf b == HS.get_tip h0)
+  = B.alloca_of_list l
 
-let length (s: t_Slice 'a): usize = sz (Seq.length s)
-let contains (#t: eqtype) (s: t_Slice t) (x: t): bool = Seq.mem x s
+// let to_list (#t:Type) (s: t_Slice t): list t = Seq.seq_to_list s
 
-let map_array #n (arr: t_Array 'a n) (f: 'a -> 'b): t_Array 'b n 
-  = FStar.Seq.map_seq_len f arr;
-    FStar.Seq.map_seq f arr 
+// let to_of_list_lemma t l = Seq.lemma_list_seq_bij l
+// let of_to_list_lemma t l = Seq.lemma_seq_list_bij l
+#set-options "--fuel 0 --ifuel 1 --z3rlimit 30"
+
+
+inline_for_extraction
+let length (s: t_Slice 'a)
+  : usize
+  = match s with
+  | Some s -> s.len
+  | None -> 0ul
+    
+unfold let spec_length (s: t_Slice 'a): GTot usize 
+  = match s with
+  | Some s -> B.len s.buffer
+  | None -> 0ul
+
+let arr_contains_spec (#t: eqtype) (s: t_Array t 'l) (x: t): Type0 = admit ()
+let contains_spec (#t: eqtype) (s: t_Slice t) (x: t): Type0 = admit ()
+let contains (#t: eqtype) (s: t_Slice t) (x: t): HST.St bool = admit ()
+
+// let map_array #n (arr: t_Array 'a n) (f: 'a -> 'b): t_Array 'b n 
+//   = FStar.Seq.map_seq_len f arr;
+//     FStar.Seq.map_seq f arr 
 
