proof-libs/fstar/core/Core.Ops.Index.fst
@@ -1,8 +1,14 @@
 module Core.Ops.Index
 
+include Core.Ops.Index.IndexMut
+
+module B = LowStar.Buffer
+module HS = FStar.HyperStack
+module HST = FStar.HyperStack.ST
+
 class t_Index t_Self t_Idx = {
   f_Output: Type;
   in_range: t_Self -> t_Idx -> Type0;
-  f_index: s:t_Self -> i:t_Idx{in_range s i} -> f_Output;
+  f_index: s:t_Self -> i:t_Idx{in_range s i} -> HST.St f_Output;
 }
 
