proof-libs/fstar/core/Core.Slice.fsti
@@ -2,9 +2,17 @@ module Core.Slice
 open Rust_primitives.Arrays
 open Rust_primitives.Integers
 
+open LowStar.BufferOps
+module B = LowStar.Buffer
+module HS = FStar.HyperStack
+module HST = FStar.HyperStack.ST
+
+inline_for_extraction
 let impl__len (#t: Type) (s: t_Slice t)
-  : len: usize {len == sz (Seq.length s)} = 
-  sz (Seq.length s)
+  : HST.St usize
+      // (requires (fun h -> B.live h s.len))
+      // (ensures  (fun h y h' -> h == h' /\ y == Seq.index (B.as_seq h s.len) 0)) 
+  = admit (); length s
 
 open Core.Slice.Iter
 
@@ -12,16 +20,21 @@ val impl__chunks (x: t_Slice 'a) (cs: usize): t_Chunks 'a
 
 let impl__iter (s: t_Slice 't): t_Slice 't = s
 
-val impl__chunks_exact (x: t_Slice 'a) (cs: usize): t_Slice (s: t_Slice 'a {length s == cs})
+val impl__chunks_exact (x: t_Slice 'a) (cs: usize): t_Slice (s: t_Slice 'a {spec_length s == cs})
 
 open Core.Ops.Index
 
 instance impl__index t n: t_Index (t_Slice t) (int_t n)
   = { f_Output = t;
-      in_range = (fun (s: t_Slice t) (i: int_t n) -> v i >= 0 && v i < v (length s));
-      f_index = (fun s i -> Seq.index s (v i));
+      in_range = (fun (s: t_Slice t) (i: int_t n) -> v i >= 0 && v i < v (spec_length s));
+      f_index = (fun (Some s) i -> 
+        admit ();
+        s.buffer.(i)
+      );
     }
 
-let impl__copy_from_slice #t (x: t_Slice t) (y:t_Slice t) : t_Slice t = y
+inline_for_extraction
+let impl__copy_from_slice #t (x: t_Slice t) (y:t_Slice t) : HST.St unit
+    = admit ()
 
 val impl__split_at #t (s: t_Slice t) (mid: usize): (t_Slice t * t_Slice t)
