proof-libs/fstar/rust_primitives/Rust_primitives.Hax.Monomorphized_update_at.fst
@@ -3,40 +3,88 @@ module Rust_primitives.Hax.Monomorphized_update_at
 open Rust_primitives
 open Rust_primitives.Hax
 open Core.Ops.Range
+open LowStar.BufferOps
+module B = LowStar.Buffer
+module HS = FStar.HyperStack
+module HST = FStar.HyperStack.ST
 
-let update_at_usize
+// let update_at_usize
+//   (s: t_Slice 't)
+//   (i: usize {i <. spec_length s}) 
+//   (v: 't)
+//   : HST.St unit//(t_Array 't (length s))
+//   = update_at s i v
+
+inline_for_extraction
+let update_array_at_usize
+  (s: t_Array 't 'l)
+  (i: usize {i <. 'l})
+  (v: 't): HST.St unit
+  = admit ();
+    s.(i) <- v
+
+inline_for_extraction    
+let update_slice_at_usize
   (s: t_Slice 't)
-  (i: usize {i <. length s}) 
-  (v: 't)
-  : t_Array 't (length s)
-  = update_at s i v
+  (i: usize {i <. spec_length s}) // {i <. 'l}) 
+  (v: 't): HST.St unit
+  = admit ();
+    (Some?.v s).buffer.(i) <- v
 
-let update_at_range #n
+let update_array_at_range #n
+  (s: t_Array 't 'n)
+  (i: t_Range (int_t n) (* TODO *))
+  (v: 't)
+  : HST.St unit
+  = admit ()
+
+let update_slice_at_range #n
   (s: t_Slice 't)
   (i: t_Range (int_t n) {(impl_index_range_slice 't n).in_range s i}) 
-  (v: t_Slice 't)
-  : t_Array 't (length s)
-  = update_at s i v
+  (v: 't)
+  : HST.St unit
+  = admit ()
   
-let update_at_range_to #n
+let update_slice_at_range_to #n
   (s: t_Slice 't)
   (i: t_RangeTo (int_t n) {(impl_index_range_to_slice 't n).in_range s i}) 
-  (v: t_Slice 't)
-  : t_Array 't (length s)
-  = update_at s i v
+  (v: 't)
+  : HST.St unit
+  = admit ()
   
-let update_at_range_from #n
+let update_array_at_range_to #n
+  (s: t_Array 't 'n)
+  (i: t_RangeTo (int_t n) (* TODO *)) 
+  (v: 't)
+  : HST.St unit
+  = admit ()
+  
+let update_slice_at_range_from #n
   (s: t_Slice 't)
   (i: t_RangeFrom (int_t n) {(impl_index_range_from_slice 't n).in_range s i}) 
-  (v: t_Slice 't)
-  : t_Array 't (length s)
-  = update_at s i v
+  (v: 't)
+  : HST.St unit
+  = admit ()
+  
+let update_array_at_range_from #n
+  (s: t_Array 't 'n)
+  (i: t_RangeFrom (int_t n) (* TODO *)) 
+  (v: 't)
+  : HST.St unit
+  = admit ()
 
-let update_at_range_full
+let update_slice_at_range_full
   (s: t_Slice 't)
   (i: t_RangeFull {(impl_index_range_full_slice 't).in_range s i}) 
   (v: t_Slice 't)
-  : t_Array 't (length s)
-  = update_at s i v
+  : HST.St unit
+  = admit ()
+
+let update_array_at_range_full
+  (s: t_Array 't 'n)
+  (i: t_RangeFull (* TODO *)) 
+  (v: 't)
+  : HST.St unit
+  = admit ()
 
 
